Added new operations for shifting by a bit-vector value, namely:
LSL: <<~
LSR: >>>~
ASR: >>~
ROR: #>>~
ROL: #<<~

These are supported by the procedures in blastLib.  For example, one can prove

w <+ 10w /\ s <+ 3w ==> w <<~ (s + 1w) <+ 73w : word16

The time-complexity is a pretty shocking but "simple" 32-bit problems seem to
be okay.  NB. ROR and ROL only bit-blast with word sizes that are a power of
two.

Added a new conversion WORD_MOD_BITS_CONV for mapping applications of
``word_mod w (n2w n)`` into ``(h -- 0) w`` where n is a power of two.

Also added support for bit-blasting arbitrary multiplication, but the word-size
limit is set to 8 bits by default.  Things seem to be just about feasible with
that limit (and become horrendously slow after that).

To improve performance, the conversion BBLAST_CONV does not have exactly the
same coverage as before.  For backward compatibility, a conversion
EBLAST_CONV (which calls SAT at every bit position) is now available.

src/n-bit/blastLib.sig
@@ -10,4 +10,8 @@ sig
     val BBLAST_TAC      : tactic
     val FULL_BBLAST_TAC : tactic
 
+    val EBLAST_CONV     : conv
+    val EBLAST_PROVE    : conv
+    val EBLAST_RULE     : rule
+    val EBLAST_TAC      : tactic
 end
